CollapsingTowers/TwoLevelBasic/Deterministic.lean
@@ -1,0 +1,33 @@
+
+import CollapsingTowers.TwoLevelBasic.SmallStep
+theorem deterministic :
+  ∀ e₀ e₁ e₂,
+    step e₀ e₁ →
+    step e₀ e₂ →
+    e₁ = e₂ :=
+  by admit
+
+theorem church_rosser :
+  ∀ e₀ l r,
+    stepn e₀ l →
+    stepn e₀ r →
+    ∃ v,
+      stepn l v ∧
+      stepn r v :=
+  by
+  intros e₀ l r Hstepl Hstepr
+  induction Hstepl generalizing r
+  case refl =>
+    exists r; constructor
+    . apply Hstepr
+    . apply stepn.refl
+  case multi le₀ le₁ le₂ IHstepl IHstepln IH =>
+    cases Hstepr
+    case refl =>
+      exists le₂; constructor
+      . apply stepn.refl
+      . apply stepn.multi; apply IHstepl; apply IHstepln
+    case multi re₀ IHstepr IHsteprn =>
+      apply IH
+      rw [deterministic _ _ _ IHstepl IHstepr]
+      apply IHsteprn
